opentheory/haskell/parser.ml
@@ -1,3 +1,171 @@
+(* ========================================================================= *)
+(* SIMPLE STREAM PARSERS IN OPENTHEORY HASKELL                               *)
+(* Joe Hurd                                                                  *)
+(* ========================================================================= *)
+
+(* ------------------------------------------------------------------------- *)
+(* Defining Haskell parsers and streams.                                     *)
+(* ------------------------------------------------------------------------- *)
+
+logfile "haskell-parser-def";;
+
+(* Streams *)
+
+let is_streamH_def =
+  let def = new_definition
+    `!(s : A stream). is_streamH s <=> T` in
+  REWRITE_RULE [] def;;
+
+let streamH_exists = prove
+  (`?(s : A stream). is_streamH s`,
+   EXISTS_TAC `s : A stream` THEN
+   REWRITE_TAC [is_streamH_def]);;
+
+let (streamH_abs_rep,streamH_rep_abs) =
+  let tybij =
+    new_type_definition
+      "streamH" ("mk_streamH","dest_streamH") streamH_exists in
+  CONJ_PAIR (REWRITE_RULE [is_streamH_def] tybij);;
+
+export_thm streamH_abs_rep;;
+export_thm streamH_rep_abs;;
+
+let streamH_tybij = CONJ streamH_abs_rep streamH_rep_abs;;
+
+let ErrorH_def = new_definition
+  `(ErrorH : A streamH) = mk_streamH Error`;;
+
+export_thm ErrorH_def;;
+
+let EofH_def = new_definition
+  `(EofH : A streamH) = mk_streamH Eof`;;
+
+export_thm EofH_def;;
+
+let StreamH_def = new_definition
+  `!(a : A) s. StreamH a s = mk_streamH (Stream a (dest_streamH s))`;;
+
+export_thm StreamH_def;;
+
+let case_streamH_def = new_definition
+  `!(e : B) b f (s : A streamH).
+     case_streamH e b f s =
+     case_stream e b (\a t. f a (mk_streamH t)) (dest_streamH s)`;;
+
+export_thm case_streamH_def;;
+
+let length_streamH_def = new_definition
+  `!(s : A streamH). length_streamH s = length_stream (dest_streamH s)`;;
+
+export_thm length_streamH_def;;
+
+let stream_to_listH_def = new_definition
+  `!(s : A streamH). stream_to_listH s = stream_to_list (dest_streamH s)`;;
+
+export_thm stream_to_listH_def;;
+
+let append_streamH_def = new_definition
+  `!l (s : A streamH).
+     append_streamH l s = mk_streamH (append_stream l (dest_streamH s))`;;
+
+export_thm append_streamH_def;;
+
+let list_to_streamH_def = new_definition
+  `!(l : A list). list_to_streamH l = mk_streamH (list_to_stream l)`;;
+
+export_thm list_to_streamH_def;;
+
+(* Parsers *)
+
+let is_parserH_def =
+  let def = new_definition
+    `!(p : (A,B) parser). is_parserH p <=> T` in
+  REWRITE_RULE [] def;;
+
+let parserH_exists = prove
+  (`?(p : (A,B) parser). is_parserH p`,
+   EXISTS_TAC `p : (A,B) parser` THEN
+   REWRITE_TAC [is_parserH_def]);;
+
+let (parserH_abs_rep,parserH_rep_abs) =
+  let tybij =
+    new_type_definition
+      "parserH" ("mk_parserH","dest_parserH") parserH_exists in
+  CONJ_PAIR (REWRITE_RULE [is_parserH_def] tybij);;
+
+export_thm parserH_abs_rep;;
+export_thm parserH_rep_abs;;
+
+let parserH_tybij = CONJ parserH_abs_rep parserH_rep_abs;;
+
+let (mk_parser_resultH_none,mk_parser_resultH_some) =
+  let def = new_definition
+    `(mk_parser_resultH : (B # A stream) option ->  (B # A streamH) option) =
+       case_option
+         NONE
+         (\ (b,s'). SOME (b, mk_streamH s'))` in
+  let th_none = prove
+    (`mk_parser_resultH (NONE : (B # A stream) option) =
+      (NONE : (B # A streamH) option)`,
+     REWRITE_TAC [def; case_option_def])
+  and th_some = prove
+    (`!(b : B) (s : A stream).
+         mk_parser_resultH (SOME (b,s)) = SOME (b, mk_streamH s)`,
+     REWRITE_TAC [def; case_option_def]) in
+  (th_none,th_some);;
+
+export_thm mk_parser_resultH_none;;
+export_thm mk_parser_resultH_some;;
+
+let mk_parser_resultH_def =
+    CONJ mk_parser_resultH_none mk_parser_resultH_some;;
+
+let (dest_parser_resultH_none,dest_parser_resultH_some) =
+  let def = new_definition
+    `(dest_parser_resultH : (B # A streamH) option ->  (B # A stream) option) =
+       case_option
+         NONE
+         (\ (b,s'). SOME (b, dest_streamH s'))` in
+  let th_none = prove
+    (`dest_parser_resultH (NONE : (B # A streamH) option) =
+      (NONE : (B # A stream) option)`,
+     REWRITE_TAC [def; case_option_def])
+  and th_some = prove
+    (`!(b : B) (s : A streamH).
+         dest_parser_resultH (SOME (b,s)) = SOME (b, dest_streamH s)`,
+     REWRITE_TAC [def; case_option_def]) in
+  (th_none,th_some);;
+
+export_thm dest_parser_resultH_none;;
+export_thm dest_parser_resultH_some;;
+
+let dest_parser_resultH_def =
+    CONJ dest_parser_resultH_none dest_parser_resultH_some;;
+
+let mk_parseH_def = new_definition
+  `!(p : A -> A stream -> (B # A stream) option).
+     mk_parseH p a s = mk_parser_resultH (p a (dest_streamH s))`;;
+
+export_thm mk_parseH_def;;
+
+let dest_parseH_def = new_definition
+  `!(p : A -> A streamH -> (B # A streamH) option).
+     dest_parseH p a s = dest_parser_resultH (p a (mk_streamH s))`;;
+
+export_thm dest_parseH_def;;
+
+let abs_parserH_def = new_definition
+  `!(p : A -> A streamH -> (B # A streamH) option).
+     abs_parserH p = mk_parserH (mk_parser (dest_parseH p))`;;
+
+export_thm abs_parserH_def;;
+
+let rep_parserH_def = new_definition
+  `!(p : (A,B) parserH).
+     rep_parserH p = mk_parseH (dest_parser (dest_parserH p))`;;
+
+export_thm rep_parserH_def;;
+
 (* ------------------------------------------------------------------------- *)
 (* A type of Haskell parsers.                                                *)
 (* ------------------------------------------------------------------------- *)
@@ -6,18 +174,59 @@ logfile "haskell-parser-src";;
 
 (* Streams *)
 
-export_haskell_thm case_stream_def;;
+let case_streamH_src = prove
+ (`(!e b (f : A -> A streamH -> B). case_streamH e b f ErrorH = e) /\
+   (!e b (f : A -> A streamH -> B). case_streamH e b f EofH = b) /\
+   (!e b (f : A -> A streamH -> B) a s.
+      case_streamH e b f (StreamH a s) = f a s)`,
+  REWRITE_TAC
+    [case_streamH_def; ErrorH_def; EofH_def; StreamH_def; case_stream_def;
+     streamH_tybij]);;
 
-export_haskell_thm length_stream_def;;
+export_haskell_thm case_streamH_src;;
 
-export_haskell_thm stream_to_list_def;;
+let length_streamH_src = prove
+ (`length_streamH (ErrorH : A streamH) = 0 /\
+   length_streamH (EofH : A streamH) = 0 /\
+   (!(a:A) s. length_streamH (StreamH a s) = length_streamH s + 1)`,
+  REWRITE_TAC
+    [length_streamH_def; ErrorH_def; EofH_def; StreamH_def; streamH_tybij;
+     length_stream_def; ADD1]);;
 
-export_haskell_thm append_stream_def;;
+export_haskell_thm length_streamH_src;;
 
-export_haskell_thm list_to_stream_def;;
+let stream_to_listH_src = prove
+ (`stream_to_listH (ErrorH : A streamH) = NONE /\
+   stream_to_listH (EofH : A streamH) = SOME [] /\
+   (!(a : A) s.
+      stream_to_listH (StreamH a s) =
+      case_option NONE (\l. SOME (CONS a l)) (stream_to_listH s))`,
+  REWRITE_TAC
+    [stream_to_listH_def; ErrorH_def; EofH_def; StreamH_def; streamH_tybij;
+     stream_to_list_def]);;
+
+export_haskell_thm stream_to_listH_src;;
+
+let append_streamH_src = prove
+ (`(!(s : A streamH). append_streamH [] s = s) /\
+   (!(h : A) t s.
+      append_streamH (CONS h t) s = StreamH h (append_streamH t s))`,
+  REWRITE_TAC
+    [append_streamH_def; streamH_tybij; StreamH_def; append_stream_def]);;
+
+export_haskell_thm append_streamH_src;;
+
+let list_to_streamH_src = prove
+ (`!(l : A list). list_to_streamH l = append_streamH l EofH`,
+  REWRITE_TAC
+    [list_to_streamH_def; streamH_tybij; EofH_def; list_to_stream_def;
+     append_streamH_def]);;
+
+export_haskell_thm list_to_streamH_src;;
 
 (* Parsers *)
 
+(***
 export_haskell_thm (CONJUNCT1 parser_tybij);;
 
 export_haskell_thm parse_def;;
@@ -67,5 +276,6 @@ export_haskell_thm list_to_stream_length;;
 export_haskell_thm stream_to_list_length;;
 
 (* Parsers *)
+***)
 
 logfile_end ();;
